Renamed good to inert.

dev/lf/tight-proof/Inert_types.v
@@ -7,72 +7,72 @@ Require Import Some_lemmas.
 Require Import Precise_flow.
 
 (* ###################################################################### *)
-(** ** Good types *)
+(** ** Inert types *)
 
-(* Definition (Good types)
+(* Definition (Inert types)
 
-A type is good if it of the form
+A type is inert if it of the form
   all(x: S)T
   rec(x: T), where T is a record type
  *)
 
-Inductive good_typ : typ -> Prop :=
-  | good_typ_all : forall S T, good_typ (typ_all S T) (* all(x: S)T *)
-  | good_typ_bnd : forall T,
+Inductive inert_typ : typ -> Prop :=
+  | inert_typ_all : forall S T, inert_typ (typ_all S T) (* all(x: S)T *)
+  | inert_typ_bnd : forall T,
       record_type T ->
-      good_typ (typ_bnd T). (* rec(x:T) *)
+      inert_typ (typ_bnd T). (* rec(x:T) *)
 
-(* Definition (Good context)
+(* Definition (Inert context)
 
-A context is good if it is of the form
+A context is inert if it is of the form
   {}
-  G, x : T where G is a good context and T is a good type *)
+  G, x : T where G is a inert context and T is a inert type *)
 
-Inductive good : ctx -> Prop :=
-  | good_empty : good empty
-  | good_all : forall pre x T,
-      good pre ->
-      good_typ T ->
+Inductive inert : ctx -> Prop :=
+  | inert_empty : inert empty
+  | inert_all : forall pre x T,
+      inert pre ->
+      inert_typ T ->
       x # pre ->
-      good (pre & x ~ T).
+      inert (pre & x ~ T).
 
-(* Good contexts bind good:
-If G |- x : T and G is a good context then T is a good type. *)
+(* Inert contexts bind inert:
+If G |- x : T and G is a inert context then T is a inert type. *)
 
-Lemma binds_good : forall G x T,
+Lemma binds_inert : forall G x T,
     binds x T G ->
-    good G ->
-    good_typ T.
+    inert G ->
+    inert_typ T.
 Proof.
-  introv Bi Hgood. induction Hgood.
+  introv Bi Hinert. induction Hinert.
   - false * binds_empty_inv.
   - destruct (binds_push_inv Bi).
     + destruct H1. subst. assumption.
-    + destruct H1. apply (IHHgood H2).
+    + destruct H1. apply (IHHinert H2).
 Qed.
 
-Lemma good_binds : forall G x T,
-    good G ->
+Lemma inert_binds : forall G x T,
+    inert G ->
     binds x T G ->
-    good_typ T.
+    inert_typ T.
 Proof.
   introv Bi Hgd.
-  eapply binds_good; eauto.
+  eapply binds_inert; eauto.
 Qed.
 
-Lemma good_typ_bnd_record : forall G x T,
-    good G ->
+Lemma inert_typ_bnd_record : forall G x T,
+    inert G ->
     binds x (typ_bnd T) G ->
     record_type T.
 Proof.
   introv Bi Hgd.
-  pose proof (good_binds Bi Hgd).
+  pose proof (inert_binds Bi Hgd).
   dependent induction H.
   assumption.
 Qed.
 
-Lemma good_unique_tight_bounds' : forall G x T T1 T2 A,
-    good_typ T ->
+Lemma inert_unique_tight_bounds' : forall G x T T1 T2 A,
+    inert_typ T ->
     precise_flow x G T (typ_rcd (dec_typ A T1 T1)) ->
     precise_flow x G T (typ_rcd (dec_typ A T2 T2)) ->
     T1 = T2.
@@ -84,8 +84,8 @@ Proof.
   - apply (record_unique_tight_bounds H Hpf1 Hpf2).
 Qed.
 
-Lemma good_unique_tight_bounds: forall G x T1 T2 A,
-  good G ->
+Lemma inert_unique_tight_bounds: forall G x T1 T2 A,
+  inert G ->
   ty_trm ty_precise sub_general G (trm_var (avar_f x)) (typ_rcd (dec_typ A T1 T1)) ->
   ty_trm ty_precise sub_general G (trm_var (avar_f x)) (typ_rcd (dec_typ A T2 T2)) ->
   T1 = T2.
@@ -95,20 +95,20 @@ Proof.
     eapply typing_implies_bound. eassumption.
   }
   destruct Bi as [T Bi].
-  pose proof (good_binds Hgd Bi) as Hgt.
+  pose proof (inert_binds Hgd Bi) as Hgt.
   pose proof (precise_flow_lemma Bi Hty1) as H1.
   pose proof (precise_flow_lemma Bi Hty2) as H2.
-  apply (good_unique_tight_bounds' Hgt H1 H2).
+  apply (inert_unique_tight_bounds' Hgt H1 H2).
 Qed.
 
-Lemma good_precise_bot : forall T G x,
-    good G ->
+Lemma inert_precise_bot : forall T G x,
+    inert G ->
     binds x T G ->
     precise_flow x G T typ_bot ->
     False.
 Proof.
   intros T G x Hgd Bis Hpf.
-  pose proof (binds_good Bis Hgd) as Hgtyp.
+  pose proof (binds_inert Bis Hgd) as Hgtyp.
   induction Hgtyp.
   - apply precise_flow_all_inv in Hpf.
     inversion Hpf.
@@ -116,25 +116,25 @@ Proof.
       inversion Contra.
 Qed.
 
-Lemma good_ty_precise_bot : forall G x,
-    good G ->
+Lemma inert_ty_precise_bot : forall G x,
+    inert G ->
     ty_trm ty_precise sub_general G (trm_var (avar_f x)) typ_bot ->
     False.
 Proof.
   intros G x Hgd Hpt.
   pose proof (typing_implies_bound Hpt) as [T Bi].
   pose proof (precise_flow_lemma Bi Hpt) as Hpf.
-  eapply good_precise_bot; eassumption.
+  eapply inert_precise_bot; eassumption.
 Qed.
 
-Lemma good_precise_sel_inv : forall G x y A,
-    good G ->
+Lemma inert_precise_sel_inv : forall G x y A,
+    inert G ->
     ty_trm ty_precise sub_general G (trm_var (avar_f x)) (typ_sel y A) ->
     False.
 Proof.
   introv Hgd Hpt.
   pose proof (typing_implies_bound Hpt) as [T Bis].
-  pose proof (good_binds Hgd Bis) as Hgt.
+  pose proof (inert_binds Hgd Bis) as Hgt.
   pose proof (precise_flow_lemma Bis Hpt) as Hpf.
   induction Hgt.
   - apply (precise_flow_all_inv) in Hpf.
@@ -142,14 +142,14 @@ Proof.
   - pose proof (precise_flow_bnd_eq_or_record H Hpf) as [[U [Contra H1]] | [ls Contra]]; inversion Contra.
 Qed.
 
-Lemma good_precise_dec_implies_record_dec : forall G x D,
-    good G ->
+Lemma inert_precise_dec_implies_record_dec : forall G x D,
+    inert G ->
     ty_trm ty_precise sub_general G (trm_var (avar_f x)) (typ_rcd D) ->
     record_dec D.
 Proof.
   introv Hgd Hpt.
   pose proof (typing_implies_bound Hpt) as [T' Bis].
-  pose proof (good_binds Hgd Bis) as Hgt.
+  pose proof (inert_binds Hgd Bis) as Hgt.
   pose proof (precise_flow_lemma Bis Hpt) as Hpf.
   induction Hgt.
   - apply (precise_flow_all_inv) in Hpf.
@@ -157,45 +157,45 @@ Proof.
   - apply (record_precise_dec_implies_record_dec H Hpf).
 Qed.
 
-Lemma good_precise_dec_typ_inv : forall G x A S U,
-    good G ->
+Lemma inert_precise_dec_typ_inv : forall G x A S U,
+    inert G ->
     ty_trm ty_precise sub_general G (trm_var (avar_f x)) (typ_rcd (dec_typ A S U)) ->
     S = U.
 Proof.
   introv Hgd Hpt.
-  pose proof (good_precise_dec_implies_record_dec Hgd Hpt) as Hrec.
+  pose proof (inert_precise_dec_implies_record_dec Hgd Hpt) as Hrec.
   inversion Hrec.
   reflexivity.
 Qed.
 
-Lemma good_precise_flow_all_inv : forall x G S T U,
-    good G ->
+Lemma inert_precise_flow_all_inv : forall x G S T U,
+    inert G ->
     precise_flow x G U (typ_all S T) ->
     U = (typ_all S T).
 Proof.
   introv Hgd Hpf.
   pose proof (precise_flow_implies_bound Hpf) as Bis.
-  pose proof (good_binds Hgd Bis) as Hgt.
+  pose proof (inert_binds Hgd Bis) as Hgt.
   dependent induction Hgt.
   - symmetry. eapply precise_flow_all_inv. eassumption.
   - pose proof (precise_flow_bnd_eq_or_record H Hpf) as [ [? [Contra _]] | [? Contra]]; inversion Contra.
 Qed.
 
-Lemma good_precise_all_inv : forall x G S T,
-    good G ->
+Lemma inert_precise_all_inv : forall x G S T,
+    inert G ->
     ty_trm ty_precise sub_general G (trm_var (avar_f x)) (typ_all S T) ->
     binds x (typ_all S T) G.
 Proof.
   introv Hgd Htyp.
   pose proof (typing_implies_bound Htyp) as [U Bi].
   pose proof (precise_flow_lemma Bi Htyp) as Hpf.
-  pose proof (good_precise_flow_all_inv Hgd Hpf) as H.
+  pose proof (inert_precise_flow_all_inv Hgd Hpf) as H.
   rewrite <- H.
   assumption.
 Qed.
 
-Lemma good_ok : forall G,
-    good G ->
+Lemma inert_ok : forall G,
+    inert G ->
     ok G.
 Proof.
   intros G HG. induction G using env_ind.
